\input{permve-ntnu-latex-assignment.tex}

\title{
\normalfont \normalsize
\textsc{Norwegian University of Science and Technology\\IT3708 -- Subsymbolic Methods in AI}
}

\author{Per Magnus Veierland\\permve@stud.ntnu.no}

\date{\normalsize\today}

\begin{document}

\fancyfoot[C]{}
\maketitle

\section*{Intelligence Emerging: EA Rank Errata Suggestion}

In the description of the rank selection in evolutionary algorithms on page 434 in section A.5.2 I've found a small error concerning the derivation in Equation A.6 and A.7.

Equation A.6 shows that Equation~\ref{eq:a6a} is equal to Equation~\ref{eq:a6b}.

\begin{equation}
\label{eq:a6a}
\sum_{i=1}^{N}\Bigg[ \text{min} + (\text{max} - \text{min})\frac{\textit{rank}(i, g) - 1}{N - 1}\Bigg]
\end{equation}

\begin{equation}
\label{eq:a6b}
N \cdot \text{min} + (\text{max} - \text{min}) \sum_{i=1}^{N}\frac{i}{N - 1}
\end{equation}

However these are not equivalent, and Equation~\ref{eq:a6b} should instead be:

\begin{equation}
N \cdot \text{min} + (\text{max} - \text{min}) \sum_{i=1}^{N}\frac{i - 1}{N - 1}
\end{equation}

This results in the following derivation, which differs from the first two steps of Equation A.7:

\begin{equation}
\sum_{i=1}^{N}\frac{i - 1}{N - 1} =
\frac{1}{N - 1}\sum_{i=1}^{N}(i - 1) =
\frac{1}{N - 1}\sum_{i=1}^{N - 1}i =
\frac{1}{N - 1} \cdot \frac{(N - 1)N}{2} =
\frac{N}{2}
\end{equation}

\end{document}

